floyd/data_at_lemmas.v
@@ -1107,7 +1107,7 @@ intros.
    apply decode_val_Vubyte_inj in H0,H1,H2,H3. subst.
    apply (predicates_hered.exp_right [Byte b0; Byte b1; Byte b2; Byte b3]).
      rewrite predicates_hered.prop_true_andp.
-      2:{ split3. reflexivity. reflexivity. apply AL. }
+      2:{ split3. reflexivity. reflexivity. split; [ | apply AL]. simpl. lia. }
   match goal with |- predicates_hered.derives ?A ?B => 
         assert (EQ: A=B); [ | rewrite EQ; apply predicates_hered.derives_refl]
     end.
@@ -1116,7 +1116,7 @@ intros.
  -
   repeat change (exp ?A) with (predicates_hered.exp A).
       normalize.normalize.
-  intros bl [? [? ?]]. simpl snd in H1.
+  intros bl [? [? [Hsize H1]]]. simpl snd in H1. simpl in Hsize.
       destruct bl as [|c0 [| c1 [| c2 [| c3 [|]]]]]; inv H.
        unfold decode_val, proj_bytes in H0. rewrite AP in H0. clear AP.
        destruct c0; try discriminate H0.
@@ -1138,7 +1138,7 @@ intros.
       normalize.normalize.
      apply predicates_hered.exp_right with [Byte b0].
      rewrite !predicates_hered.prop_true_andp by 
-     (split3; [ reflexivity |  | apply Z.divide_1_l  ];
+     (split; [ | split3]; [ reflexivity | | simpl; rep_lia | apply Z.divide_1_l  ];
      unfold decode_val, Vubyte; simpl; f_equal;
      rewrite decode_int_single;
      apply zero_ext_inrange; change (two_p _ - 1) with 255;
@@ -1413,7 +1413,7 @@ intros.
     apply decode_val_Vubyte_inj in H0,H1,H2,H3,H4,H5,H6,H7; subst.
    apply (predicates_hered.exp_right (map Byte [b0;b1;b2;b3;b4;b5;b6;b7])).
      rewrite predicates_hered.prop_true_andp.
-      2:{ split3. reflexivity. reflexivity. apply AL. }
+      2:{ split3. reflexivity. reflexivity. split. simpl; lia. apply AL. }
    rewrite address_mapsto_8bytes_aux; auto.
 Qed.
 
@@ -1722,7 +1722,7 @@ Proof.
     2:{ split3. reflexivity. unfold decode_val. simpl.
         f_equal. apply zero_ext_16. 
         pose proof (decode_int_range [b0; b1]). simpl in H.
-        assert (two_power_pos 16 = 65536) by reflexivity. lia. apply AL. 
+        assert (two_power_pos 16 = 65536) by reflexivity. lia. split. simpl; lia. apply AL. 
       }
   match goal with |- predicates_hered.derives ?A ?B => 
         assert (EQ: A=B); [ | rewrite EQ; apply predicates_hered.derives_refl]
@@ -1730,8 +1730,8 @@ Proof.
   apply address_mapsto_2bytes_aux; auto.
  - repeat change (exp ?A) with (predicates_hered.exp A).
    normalize.normalize.
-   intros bl [? [? ?]].
-    simpl snd in H1.
+   intros bl [? [? [Hsize ?]]].
+    simpl snd in H1. simpl in Hsize.
    destruct bl as [|c0 [| c1 [| c2 [| c3 [|]]]]]; inv H.
    unfold decode_val, proj_bytes in H0.
    destruct c0; try solve [destruct Archi.ptr64 eqn:AP; discriminate].
@@ -1748,7 +1748,7 @@ Proof.
   normalize.normalize.
   apply predicates_hered.exp_right with [Byte b0].
   rewrite !predicates_hered.prop_true_andp by 
- (split3; [ reflexivity |  | apply Z.divide_1_l  ];
+ (split; [ | split3]; [ reflexivity |  | simpl; rep_lia | apply Z.divide_1_l  ];
  unfold decode_val, Vubyte; simpl; f_equal;
  rewrite decode_int_single;
  apply zero_ext_inrange; change (two_p _ - 1) with 255;
